Just a bit of thinking out loudly on when a linux router is equivalent to something that does not touch the mac-layer.

thy/Routing/LinuxRouter.thy
@@ -5,6 +5,7 @@ imports
 	"../Simple_Firewall/SimpleFw_Semantics"
 	(* for the simple packet extension *)
 	"../OpenFlow/OpenFlowMatches"
+	"~~/src/HOL/Library/Monad_Syntax"
 begin
 definition "fromMaybe a m = (case m of Some a \<Rightarrow> a | None \<Rightarrow> a)" (* mehr Haskell wagen *)
 
@@ -24,27 +25,23 @@ Oversimplified linux router:
 record interface =
 	iface_name :: string
 	iface_mac :: "48 word"
-	(*iface_ips :: "(ipv4addr \<times> 32 prefix_match) set" (* there is a set of IP addresses and the reachable subnets for them *), but we don't use that right now, so it is commented out *)
+	(*iface_ips :: "(ipv4addr \<times> 32 prefix_match) set" (* there is a set of IP addresses and the reachable subnets for them *), but we don't use that right now, so it is commented out. 
+	Also, part of that information is already in the routing table, so careful here\<dots> *)
 
 definition iface_packet_check ::  "interface list \<Rightarrow> 'b simple_packet_ext_scheme \<Rightarrow> interface option"
 where "iface_packet_check ifs p \<equiv> find (\<lambda>i. iface_name i = p_iiface p \<and> iface_mac i = p_l2dst p) ifs" 
 term simple_fw
-definition simple_linux_router :: "routing_rule list \<Rightarrow> simple_rule list \<Rightarrow> (32 word \<Rightarrow> 48 word) \<Rightarrow> interface list \<Rightarrow> simple_packet_ext \<Rightarrow> simple_packet_ext option" where
-"simple_linux_router rt fw mlf ifl p \<equiv> (
-case iface_packet_check ifl p of
-   	None \<Rightarrow> None |
-   	Some i \<Rightarrow>
-   		(let
-		rd = routing_table_semantics rt (p_dst p);
-		p = p_oiface_update (const (output_iface rd)) p;
-		fd = simple_fw fw p;
-		nh = fromMaybe (p_dst p) (next_hop rd);
-		ma = mlf nh
-		in case fd of
-			Decision FinalAllow \<Rightarrow> Some (p_oiface_update (const (output_iface rd)) p) |
-			Decision FinalDeny \<Rightarrow> None
-	)
-)"
+definition simple_linux_router :: "routing_rule list \<Rightarrow> simple_rule list \<Rightarrow> (32 word \<Rightarrow> 48 word option) \<Rightarrow> interface list \<Rightarrow> simple_packet_ext \<Rightarrow> simple_packet_ext option" where
+"simple_linux_router rt fw mlf ifl p \<equiv> do {
+	_ \<leftarrow> iface_packet_check ifl p;
+	let rd = routing_table_semantics rt (p_dst p);
+	let p = p_oiface_update (const (output_iface rd)) p;
+	let fd = simple_fw fw p;
+	let nh = fromMaybe (p_dst p) (next_hop rd);
+	ma \<leftarrow> mlf nh;
+	_ \<leftarrow> (case fd of Decision FinalAllow \<Rightarrow> Some () | Decision FinalDeny \<Rightarrow> None);
+	Some (p_l2dst_update (const ma) p)
+}"
 (* Can I find something that looks a bit more semantic. Maybe the option monad can reduce a bit of the foo? *)
 (* TODO: What happens in linux, if I send a packet to an interface with the mac of another interface? Hopefully, that is going to be dropped? *) 
 
@@ -54,5 +51,70 @@ case iface_packet_check ifl p of
  - Only default iptables table (no raw, nat)
  - No traffic to localhost (might be a limit to lift\<dots>)
 *)
+
+text{* Transformed linux router: does not do layer 2 modifications and throws away packets that would leave on the same interface that they came in on. 
+ The entire idea is that @{term iface_packet_check} will only fail if the packet is bound for someone else on that subnet, so the routing decision would, if applied, just output the packet where it came from.*}
+definition simple_linux_router_nomac :: "routing_rule list \<Rightarrow> simple_rule list \<Rightarrow> 'a simple_packet_scheme \<Rightarrow> 'a simple_packet_scheme option" where
+"simple_linux_router_nomac rt fw p \<equiv> do {
+   		let rd = routing_table_semantics rt (p_dst p);
+   		_ \<leftarrow> (if output_iface rd = p_oiface p then None else Some ());
+		let p = p_oiface_update (const (output_iface rd)) p;
+		let fd = simple_fw fw p;
+		_ \<leftarrow> (case fd of Decision FinalAllow \<Rightarrow> Some () | Decision FinalDeny \<Rightarrow> None);
+		Some p
+}"
+(* an alternative formulation would maybe be "if the routing decision for the source is the same as for the destination, don't forward it." 
+   This might be advantageous in $cases, however, this formulation is clearly easier to translate *)
+
+lemma rtr_nomac_e1:
+	assumes "simple_linux_router rt fw mlf ifl pi = Some po"
+	assumes "simple_linux_router_nomac rt fw pi = Some po'"
+	shows "\<exists>x. po = p_l2dst_update x po'"
+using assms
+unfolding simple_linux_router_nomac_def simple_linux_router_def
+by(simp add: Let_def split: option.splits state.splits final_decision.splits Option.bind_splits if_splits) blast+
+
+lemma rtr_nomac_e2:
+	assumes "simple_linux_router rt fw mlf ifl pi = Some po"
+	assumes "p_oiface pi \<noteq> p_oiface po"
+	shows "\<exists>po'. simple_linux_router_nomac rt fw pi = Some po'"
+using assms
+unfolding simple_linux_router_nomac_def simple_linux_router_def
+by(clarsimp simp add: Let_def const_def split: option.splits state.splits final_decision.splits Option.bind_splits if_splits)
+
+lemma rtr_nomac_e3:
+	assumes "simple_linux_router_nomac rt fw pi = Some po"
+	assumes "iface_packet_check ifl pi = Some i(*don'tcare*)"
+	assumes "mlf (fromMaybe (p_dst pi) (next_hop (routing_table_semantics rt (p_dst pi)))) = Some i2"
+	shows "\<exists>po'. simple_linux_router rt fw mlf ifl pi = Some po'"
+using assms
+unfolding simple_linux_router_nomac_def simple_linux_router_def
+by(clarsimp simp add: Let_def const_def split: option.splits state.splits final_decision.splits Option.bind_splits if_splits)
+
+lemma rtr_nomac_eq:
+	assumes "iface_packet_check ifl pi = None \<longleftrightarrow> output_iface (routing_table_semantics rt (p_dst pi)) = p_oiface pi"
+	assumes "mlf (fromMaybe (p_dst pi) (next_hop (routing_table_semantics rt (p_dst pi)))) = Some i2"
+	shows "\<exists>x. map_option (p_l2dst_update x) (simple_linux_router_nomac rt fw pi) = simple_linux_router rt fw mlf ifl pi"
+proof(cases "simple_linux_router_nomac rt fw pi"; cases "simple_linux_router rt fw mlf ifl pi")
+	case goal4
+	note rtr_nomac_e1[OF goal4(2) goal4(1)]
+	with goal4 show ?case by auto 
+next
+	case (goal2 a)
+	from goal2(2) have "iface_packet_check ifl pi \<noteq> None" by(simp add: simple_linux_router_def Let_def const_def split: option.splits state.splits final_decision.splits Option.bind_splits if_splits) 
+	hence "p_oiface pi \<noteq> p_oiface a" using assms(1) goal2(2) by(clarsimp simp add: simple_linux_router_def Let_def const_def split: option.splits state.splits final_decision.splits Option.bind_splits if_splits)
+	note rtr_nomac_e2[OF goal2(2) this]
+	with goal2(1) have False by simp
+	thus ?case ..
+next
+	case (goal3 a)
+	from goal3(1) have "p_oiface pi \<noteq> p_oiface a" 
+		by(clarsimp simp add: simple_linux_router_nomac_def Let_def const_def split:  state.splits final_decision.splits if_splits Option.bind_splits) (* woha, the order of the splits is important\<dots> *) 
+	hence "iface_packet_check ifl pi \<noteq> None" using goal3(1) by(clarsimp simp add: simple_linux_router_nomac_def Let_def const_def assms split:  state.splits final_decision.splits if_splits Option.bind_splits)
+	then obtain i3 where "iface_packet_check ifl pi = Some i3" by blast
+	note rtr_nomac_e3[OF goal3(1) this] assms(2)
+	with goal3(2) have False by force
+	thus ?case ..
+qed simp
 
 end
